LeanLinq/Driver/Mssql.lean
@@ -245,5 +245,6 @@ where
     | _, _, .seq g x => do Pure.pure ((← go g) (← go x))
     | _, _, .bind x k => do go (k (← go x))
     | _, _, .forAll xs f => xs.mapM fun a => go (f a)
+    | _, _, .bindD x f _ _ => do go (f (← go x))
 
 end LeanLinq
